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Question 2

Part 4.

Proof. In this question , based on the condition that f being a bijection, we are required to
show that

f−1(C1 ∩ C2) = f−1(C1) ∩ f−1(C2)

Step 1. Verify that f−1(C1 ∩ C2) ⊂ f−1(C1) ∩ f−1(C2)
∀x ∈ f−1(C1 ∩ C2), we have: ∃y ∈ C1 ∩ C2 s.t. x = f−1(y)
So, y ∈ C1 and y ∈ C2 s.t. x = f−1(y)
So, y ∈ C1 s.t. x = f−1(y) and y ∈ C2 s.t. x = f−1(y)
So, x ∈ f−1(C1) and x ∈ f−1(C2)
So, x ∈ f−1(C1) ∩ f−1(C2)
In this way, we showed that f−1(C1 ∩ C2) ⊂ f−1(C1) ∩ f−1(C2)
Step 2. Verify that f−1(C1) ∩ f−1(C2) ⊂ f−1(C1 ∩ C2)
∀x ∈ f−1(C1) ∩ f−1(C2), we have: x ∈ f−1(C1) and x ∈ f−1(C2)
So, ∃y1 ∈ C1 s.t. x = f−1(y1) and ∃y2 ∈ C2 s.t. x = f−1(y2)
Since f−1 is a bijection, which means f−1 is one-to-one. Since f−1(y1) = x = f−1(y2), by

the de�nition of one-to-one function, we must have: y1 = y2.
y := y1 = y2, so we have: y ∈ C1 ∩ C2 and x = f−1(y)
So, ∃y ∈ C1 ∩ C2, s.t. x = f−1(y), i.e., x ∈ f−1(C1 ∩ C2)
In this way, we showed that f−1(C1) ∩ f−1(C2) ⊂ f−1(C1 ∩ C2) �

Question 4

Part 1.

Proof. ∀x, y ∈ S1∩S2∩ ...∩Sn, ∀α, β ∈ R, we need to verify that αx+βy ∈ S1∩S2∩ ...∩Sn

Since S1, ..., Sn are all linear subspaces, we have: αx+βy ∈ S1,αx+βy ∈ S2, ..., αx+βy ∈
Sn, which means αx+ βy ∈ S1 ∩ S2 ∩ ... ∩ Sn �

Part 2

Proof. Consider the counter example:

S1 := span

([
0
1

])
=

{[
0
x

]
: x ∈ R

}
S1 := span

([
1
0

])
) =

{[
y
0

]
: y ∈ R

}
It is obvious that S1 and S2 are all linear subspaces of R2(Prove it by the de�nition of

linear subspace).

In this case, S1∪S2 =

{[
0
x

]
: x ∈ R

}
∪
{[

y
0

]
: y ∈ R

}
. In particular, a typical element

of S1 ∪ S2 is an element in R2 that must have at least one coordinate being 0.
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However, ∀α, β ∈ R with α, β 6= 0, we have α

[
0
1

]
+ β

[
1
0

]
=

[
α
β

]
/∈ S1 ∪ S2 since

both coordinates of the vector

[
α
β

]
are not 0.

This tells us that S1 ∪ S2 is not a linear subspace of R2 since

[
0
1

]
∈ S1 ⊂ S1 ∪ S2 and[

1
0

]
∈ S2 ⊂ S1 ∪ S2 �


